replace_range - ...미치겠네;; 야, 여기서 왜 타입 체크에 실패하냐?

src/study/Nemonuri.Study.CSharpSyntaxRewriter2.Modifier2/Nemonuri.StratifiedNodes.Common.fst
@@ -6,6 +6,11 @@ module L = FStar.List.Tot
 let aggregator (t:Type) = (aggregated:t) -> (aggregating:t) -> t
 //---|
 
+//--- predicates ---
+let filter_theorem (#a: Type) (f: (a -> Tot bool)) (l: list a) : prop =
+  forall x. L.memP x (L.filter f l) <==> L.memP x l /\ f x
+//---|
+
 //--- theory members ---
 // https://learn.microsoft.com/en-us/dotnet/api/system.linq.enumerable.skipwhile?view=net-9.0
 let rec skip_while #t
@@ -44,5 +49,15 @@ let rec find_index #t
   match predicate hd with
   | true -> 0
   | false -> 1 + (find_index tl predicate)
+
+// https://github.com/FStarLang/FStar/blob/master/ulib/FStar.List.Tot.Base.fst
+(*
+let filter (#a: Type) (f: (a -> Tot bool)) (l: list a)
+  : Pure (list a) True 
+         (ensures fun _ -> filter_theorem f l)
+  =
+  L.filter f l
+*)
+
 
 //---|
