src/study/Nemonuri.Study.CSharpSyntaxRewriter2.Modifier2/Nemonuri.StratifiedNodes.Factories.NodeLists.fst
@@ -1,0 +1,103 @@
+module Nemonuri.StratifiedNodes.Factories.NodeLists
+
+module L = FStar.List.Tot
+module I = Nemonuri.StratifiedNodes.Internals
+module N = Nemonuri.StratifiedNodes.Nodes
+module C = Nemonuri.StratifiedNodes.Children
+module Id = Nemonuri.StratifiedNodes.Indexes
+module E = Nemonuri.StratifiedNodes.Nodes.Equivalence
+module Common = Nemonuri.StratifiedNodes.Common
+module Fn = Nemonuri.StratifiedNodes.Factories.Nodes
+
+//--- theory members ---
+
+// https://learn.microsoft.com/en-us/dotnet/api/microsoft.codeanalysis.syntaxlist-1?view=roslyn-dotnet-4.12.0
+// https://github.com/dotnet/roslyn/blob/main/src/Compilers/Core/Portable/Syntax/SyntaxList%601.cs
+
+let insert_range #t 
+  (node_list:N.node_list t) 
+  (index:nat{ index <= L.length node_list })
+  (inserting_node_list:N.node_list t)
+  : Tot (N.node_list t)
+  =
+  let (l1, l2) = L.splitAt index node_list in
+  let l3 = L.append l1 inserting_node_list in
+  L.append l3 l2
+
+let insert #t
+  (node_list:N.node_list t) 
+  (index:nat{ index <= L.length node_list })
+  (inserting_node:N.node t)
+  : Tot (N.node_list t)
+  =
+  insert_range node_list index [inserting_node]
+
+
+let add_range #t
+  (node_list:N.node_list t) 
+  (inserting_node_list:N.node_list t)
+  : Tot (N.node_list t)
+  =
+  insert_range node_list (L.length node_list) inserting_node_list
+
+let add #t
+  (node_list:N.node_list t) 
+  (inserting_node:N.node t)
+  : Tot (N.node_list t)
+  =
+  insert node_list (L.length node_list) inserting_node
+
+
+let remove_all #t 
+  (node_list: N.node_list t)
+  (exclusion_predicate: (N.node t) -> Tot bool) 
+  : Pure (N.node_list t) True
+    (ensures fun _ -> Common.filter_theorem exclusion_predicate node_list)
+  =
+  L.mem_filter_forall exclusion_predicate node_list;
+  L.filter exclusion_predicate node_list
+
+let rec remove_first #t 
+  (node_list:N.node_list t) (exclusion_predicate: (N.node t) -> Tot bool)
+  : Tot (N.node_list t) (decreases node_list)
+  =
+  match node_list with
+  | [] -> []
+  | hd::tl ->
+  match (exclusion_predicate hd) with
+  | false -> tl
+  | true -> hd::(remove_first tl exclusion_predicate)
+
+let remove #t (node_list:N.node_list t) (node:N.node t)
+  : Tot (N.node_list t)
+  =
+  remove_first node_list (op_disEquality node)
+
+let remove_at #t (node_list:N.node_list t) (index:nat{ index < L.length node_list })
+  : Tot (N.node_list t)
+  =
+  remove node_list (L.index node_list index)
+
+
+let replace_range_at #t 
+  (node_list:N.node_list t) 
+  (index:nat{ index < L.length node_list })
+  (inserting_node_list:N.node_list t)
+  : Tot (N.node_list t)
+  =
+  let v1 = remove_at node_list index in
+  insert_range node_list index inserting_node_list
+
+
+let replace_range #t
+  (node_list:N.node_list t) 
+  (node:N.node t) //{ L.contains node node_list }
+  (inserting_node_list:N.node_list t)
+  : Tot (N.node_list t)
+  =
+  assume (Some? (N.try_get_first_index_of_predicate node_list (op_Equality node)));
+  let Some index = N.try_get_first_index_of_predicate node_list (op_Equality node) in
+  replace_range_at node_list index inserting_node_list
+
+
+//---|
