src/study/Nemonuri.Study.CSharpSyntaxRewriter2.Modifier2/Nemonuri.StratifiedNodes.Factories.Nodes.fst
@@ -1,0 +1,85 @@
+module Nemonuri.StratifiedNodes.Factories.Nodes
+
+module L = FStar.List.Tot
+module I = Nemonuri.StratifiedNodes.Internals
+module N = Nemonuri.StratifiedNodes.Nodes
+module C = Nemonuri.StratifiedNodes.Children
+module Id = Nemonuri.StratifiedNodes.Indexes
+module E = Nemonuri.StratifiedNodes.Nodes.Equivalence
+module Common = Nemonuri.StratifiedNodes.Common
+
+//--- theory members ---
+
+let is_leaf_and_has_value #t (node:N.node t) (value:t)
+  : Tot bool =
+  (N.get_value node = value) && (N.is_leaf node)
+
+let create_leaf_node (#t:eqtype) (value:t)
+  : Pure (N.node t) 
+         (requires True) 
+         (ensures fun r -> is_leaf_and_has_value r value)
+  =
+  N.to_node (I.SNode (I.SNil) value)
+
+
+let is_equal_to_result_of_create_leaf_node_if_node_is_leaf #t (node:N.node t) (value:t)
+  : Tot bool =
+  (N.get_value node = value) && (
+    match N.is_leaf node with
+    | true -> (create_leaf_node value) = node
+    | false -> true
+  )
+
+let replace_value #t (node:N.node t) (value:t)
+  : Pure (N.node t) 
+         (requires True) 
+         (ensures fun r -> is_equal_to_result_of_create_leaf_node_if_node_is_leaf r value)
+  =
+  let internal = node.internal in
+  let new_internal = I.SNode internal.children value in
+  N.to_node new_internal
+
+let replace_children #t (node:N.node t) (children:N.node_list t)
+  : Pure (N.node t) 
+         (requires True)
+         (ensures fun r -> E.are_equivalent_as_node_list children r.internal.children)
+(*
+         (ensures fun node -> 
+           ((I.get_list_level node.internal.children) = (I.get_list_level (N.to_node_list_inverse children))) &&
+           (node.internal.children = (N.to_node_list_inverse children)) &&
+           ((N.get_list_level (N.get_children node)) = (N.get_list_level children)) &&
+           ((N.get_children node) = children)
+         )
+*)
+  =
+  let internal = node.internal in
+  let new_internal = I.SNode (N.to_node_list_inverse children) internal.value in
+  N.to_node new_internal
+
+
+let create_node (#t:eqtype) (value:t) (children:N.node_list t)
+  : Tot (N.node t) =
+  let node = create_leaf_node value in
+  match children with
+  | [] -> node
+  | _ -> replace_children node children
+
+
+
+//---|
+
+
+//--- propositions ---
+
+//---|
+
+//#push-options "--query_stats"
+//#pop-options
+
+// normalized 된 결과를 볼 수 있나?
+(*
+let assert1 = assert ( forall (t:eqtype) (value:t) (children:N.node_list t). 
+    let n = (create_node value children) in
+    (n = (create_leaf_node value)) || (n = replace_children (create_leaf_node value) children) 
+  ) by FStar.Tactics.V2.compute()
+*)
